syntax/SLoopUnroll.v
@@ -14,3 +14,17 @@ Definition peel_unroll : nat -> SPolIRs.Loop.t -> SPolIRs.Loop.t :=
 
 Definition peel_unroll_changed : nat -> SPolIRs.Loop.t -> bool :=
   CoreUnroll.peel_unroll_changed.
+
+Definition peel_plan : Type :=
+  CoreUnroll.peel_plan.
+
+Definition prefix_peel_plan : nat -> SPolIRs.Loop.expr -> peel_plan :=
+  CoreUnroll.prefix_peel_plan.
+
+Definition check_peel_plan : SPolIRs.Loop.expr -> SPolIRs.Loop.expr -> peel_plan -> bool :=
+  CoreUnroll.check_peel_plan.
+
+Definition checked_lower_peel_plan_stmt :
+    peel_plan -> SPolIRs.Loop.expr -> SPolIRs.Loop.expr -> SPolIRs.Loop.stmt ->
+    option SPolIRs.Loop.stmt :=
+  CoreUnroll.checked_lower_peel_plan_stmt.
